theories/Normalization.v
@@ -1,5 +1,5 @@
 (******************************************************************************)
-(*   Copyright (c) 2019--2021 - Paulo Torrens <paulotorrens AT gnu DOT org>   *)
+(*   Copyright (c) 2019--2022 - Paulo Torrens <paulotorrens AT gnu DOT org>   *)
 (******************************************************************************)
 
 Require Import Lia.
